Finish the first version of in-place reversal of a list

Reversal.thy
@@ -3,22 +3,37 @@ imports VCG
 begin
 
 locale list_rev_example =
-fixes i::string and j::string and k::string
+fixes i::string and j::string and k::string and it::int
 begin
 
 abbreviation update_mem
   where "update_mem f s \<equiv> State (f (mem s)) (vars s)"
 
+abbreviation init where
+"init \<equiv> BASIC (\<lambda>s. update_mem (\<lambda>m . m((vars s) j := 0, it := (vars s) i)) s)"
+
 abbreviation list_rev where
-"list_rev \<equiv> 
-  BASIC (\<lambda> s . let loc_j = (vars s) j in update_mem (\<lambda> m . m(loc_j := 0)) s)"
+"list_rev \<equiv> BASIC (\<lambda>s. update_mem (\<lambda>m . m((vars s) k := (mem s) ((vars s) i + 1), (mem s) ((vars s) i + 1) := (vars s) j, (vars s) j := (vars s) i, (vars s) i := (vars s) k)) s)"
 
-abbreviation pre0::"assn" where "pre0 \<equiv> \<lambda>s. \<exists>\<alpha> \<beta>. (list s \<alpha> i) \<and> (list s \<beta> j) \<and> (rev \<alpha> = (append (rev \<alpha>) \<beta>))"
+abbreviation pre0::"assn" where "pre0 \<equiv> \<lambda>s. \<exists>\<alpha> \<beta>. (list s \<alpha> ((vars s) i)) \<and> (list s \<beta> ((vars s) j)) \<and> (rev \<alpha> = (append (rev \<alpha>) \<beta>)) \<and> 
+  (\<forall>k::string. (reach s ((vars s) i) ((vars s) k)) \<and> (reach s ((vars s) j) ((vars s) k)) \<longrightarrow> ((vars s) k = 0))"
 
-abbreviation loopcom::"newstate \<Rightarrow> newstate" where 
-"loopcom \<equiv> \<lambda>s. s(k := s (i + 1), s (i + 1) := j, j := i, i := k)"
+abbreviation inv::"assn" where "inv \<equiv> \<lambda>s. \<exists>\<alpha> \<beta> \<alpha>\<^sub>0. (list s \<alpha> ((vars s) i)) \<and> (list s \<beta> ((vars s) j))  \<and> (list s \<alpha>\<^sub>0 it) \<and> (rev \<alpha>\<^sub>0 = (append (rev \<alpha>) \<beta>)) \<and> 
+  (\<forall>k::string. (reach s ((vars s) i) ((vars s) k)) \<and> (reach s ((vars s) j) ((vars s) k)) \<longrightarrow> ((vars s) k = 0))"
 
-abbreviation revers::
+abbreviation post::"assn" where "post \<equiv> \<lambda>s. \<exists>\<alpha> \<beta> \<alpha>\<^sub>0. (list s \<alpha> ((vars s) i)) \<and> (list s \<beta> ((vars s) j)) \<and> (list s \<alpha>\<^sub>0 it) \<and> (rev \<alpha>\<^sub>0 = (append (rev \<alpha>) \<beta>)) \<and> 
+  (\<forall>k::string. (reach s ((vars s) i) ((vars s) k)) \<and> (reach s ((vars s) j) ((vars s) k)) \<longrightarrow> ((vars s) k = 0))"
+
+abbreviation loopcom::com where 
+"loopcom \<equiv> init;; WHILE (\<lambda>s. (vars s) i \<noteq> 0) INV inv DO list_rev OD"
+
+lemma "\<turnstile>\<^sub>t\<^sub>r {pre0} loopcom {post}"
+apply(rule Seq)
+prefer 2
+apply(rule While [where P = inv])
+apply simp
+sorry
 
 end
+
 end
