Ann_Com.thy
@@ -5,7 +5,7 @@ begin
 type_synonym address = int
 type_synonym memory = "address \<Rightarrow> int"
 datatype newstate = 
-  State (mem: "address \<Rightarrow> int") (vars: "string \<Rightarrow> int")
+  State (mem: "address \<Rightarrow> int") (vars: "string \<Rightarrow> address")
 
 type_synonym assn = "newstate \<Rightarrow> bool"
 
@@ -18,12 +18,8 @@ datatype com =
 
 fun list :: "newstate \<Rightarrow> (int list) \<Rightarrow> int \<Rightarrow> bool" where 
 "list s [] i = (i = (0::int))"|
-"list s (x#xs) i = (\<exists>j. ((mem s) i = j) \<and> ((mem s) (i+1) = x) \<and> list s xs j)"
+"list s (x#xs) i = (\<exists>j. ((mem s) i = x) \<and> ((mem s) (i + 1) = j) \<and> list s xs j)"
 
-(* s where "s \<equiv> \<lambda> i . if i = 1 then 3 else (if i = 2 then 42 else (if i = 3 then 0 else 43))"
-
-lemma "list s [42, 43] 1" by force
-*)
 fun reach_step::"newstate \<Rightarrow> nat \<Rightarrow> int \<Rightarrow> int \<Rightarrow> bool" where
 "reach_step s 0 i j = (i = j)"|
 "reach_step s (Suc n) i j = (\<exists>a k. ((mem s) i = a) \<and> ((mem s) (i + 1) = k) \<and> (reach_step s n k j))"
